feat: multiple Lean contexts for code examples

static/bindings.js
@@ -3,15 +3,20 @@ window.onload = () => {
     for (const c of document.querySelectorAll(".hl.lean .token")) {
         if (c.dataset.binding != "") {
             c.addEventListener("mouseover", (event) => {
-                for (const tok of c.closest(".hl.lean").querySelectorAll(".token")) {
-                    if (c.dataset.binding == tok.dataset.binding) {
-                        tok.classList.add("binding-hl");
+                const context = c.closest(".hl.lean").dataset.leanContext;
+                for (const example of document.querySelectorAll(".hl.lean")) {
+                    if (example.dataset.leanContext == context) {
+                        for (const tok of example.querySelectorAll(".token")) {
+                            if (c.dataset.binding == tok.dataset.binding) {
+                                tok.classList.add("binding-hl");
+                            }
+                        }
                     }
                 }
             });
         }
         c.addEventListener("mouseout", (event) => {
-            for (const tok of c.closest(".hl.lean").querySelectorAll(".token")) {
+            for (const tok of document.querySelectorAll(".hl.lean .token")) {
                 tok.classList.remove("binding-hl");
             }
         });
