LeanDoc/Genre.lean
@@ -85,22 +85,30 @@ def page_link : RoleExpander
     pure #[val]
   | _, _ => throwUnsupportedSyntax
 
-open LeanDoc.Genre.Highlighted in
-@[code_block_expander lean]
-def lean : CodeBlockExpander
-  | _, str => do
-    -- FIXME this is a horrid kludge - find a way to systematically rewrite srclocs?
-    let preString := (← getFileMap).source.extract 0 (str.raw.getPos?.getD 0)
-    let inputString := Id.run do
-      let mut code := ""
-      let mut iter := preString.iter
-      while !iter.atEnd do
-        if iter.curr == '\n' then code := code.push '\n'
-        else code := code.push ' '
-        iter := iter.next
-      code := code ++ str.getString
-      return code
-    let context := Parser.mkInputContext inputString "<example>"
+structure ExampleContext where
+  contexts : NameMap (Command.State × Parser.ModuleParserState) := {}
+deriving Inhabited
+
+initialize exampleContextExt : EnvExtension ExampleContext ← registerEnvExtension (pure {})
+
+-- FIXME this is a horrid kludge - find a way to systematically rewrite srclocs?
+def parserInputString [Monad m] [MonadFileMap m] (str : TSyntax `str) : m String := do
+  let preString := (← getFileMap).source.extract 0 (str.raw.getPos?.getD 0)
+  let mut code := ""
+  let mut iter := preString.iter
+  while !iter.atEnd do
+    if iter.curr == '\n' then code := code.push '\n'
+    else
+      for _ in [0:iter.curr.utf8Size.toNat] do
+        code := code.push ' '
+    iter := iter.next
+  code := code ++ str.getString
+  return code
+
+@[code_block_expander leanInit]
+def leanInit : CodeBlockExpander
+  | #[.anonymous (.name x)], str => do
+    let context := Parser.mkInputContext (← parserInputString str) "<example>"
     let (header, state, msgs) ← Parser.parseHeader context
     initializeLeanContext
     let opts := Options.empty -- .setBool `trace.Elab.info true
@@ -110,15 +118,30 @@ def lean : CodeBlockExpander
         logMessage msg
       liftM (m := IO) (throw <| IO.userError "Errors during import; aborting")
     let commandState := configureCommandState env msgs
-    let s ← IO.processCommands context state commandState
-    if let some expectedEnd := str.raw.getTailPos? then
-      -- TODO compare code points instead of UTF8
-      if s.parserState.pos < expectedEnd then
-        dbg_trace "ended at {(← getFileMap).utf8PosToLspPos s.parserState.pos} {s.commands}"
+    modifyEnv <| fun env => exampleContextExt.modifyState env fun s => {s with contexts := s.contexts.insert x.getId (commandState, state)}
+    pure #[]
+  | otherArgs, _ => dbg_trace "Didn't understand {repr otherArgs}"; throwUnsupportedSyntax
+where
+  initializeLeanContext : IO Unit := do
+    let leanPath ← Lean.findSysroot
+    Lean.initSearchPath leanPath
+  configureCommandState (env : Environment) (msg : MessageLog) : Command.State :=
+    { Command.mkState env msg with infoState := { enabled := true } }
+
+open LeanDoc.Genre.Highlighted in
+@[code_block_expander lean]
+def lean : CodeBlockExpander
+  | #[.anonymous (.name x)], str => do
+    let some (commandState, state) := exampleContextExt.getState (← getEnv) |>.contexts.find? x.getId
+      | throwErrorAt x "Can't find example context"
+    let context := Parser.mkInputContext (← parserInputString str) "<example>"
+    -- Process with empty messages to avoid duplicate output
+    let s ← IO.processCommands context state { commandState with messages.msgs := {} }
     for t in s.commandState.infoState.trees do
       pushInfoTree t
     for msg in s.commandState.messages.msgs do
       logMessage msg
+    modifyEnv <| fun env => exampleContextExt.modifyState env fun st => {s with contexts := st.contexts.insert x.getId (s.commandState, s.parserState)}
     let mut hls := Highlighted.empty
     let infoSt ← getInfoState
     let env ← getEnv
@@ -130,13 +153,8 @@ def lean : CodeBlockExpander
     finally
       setInfoState infoSt
       setEnv env
-    pure #[← ``(Block.other (Blog.BlockExt.highlightedCode $(quote hls)) #[Block.code none #[] 0 $(quote str.getString)])]
-where
-  initializeLeanContext : IO Unit := do
-    let leanPath ← Lean.findSysroot
-    Lean.initSearchPath leanPath
-  configureCommandState (env : Environment) (msg : MessageLog) : Command.State :=
-    { Command.mkState env msg with infoState := { enabled := true } }
+    pure #[← ``(Block.other (Blog.BlockExt.highlightedCode $(quote x.getId) $(quote hls)) #[Block.code none #[] 0 $(quote str.getString)])]
+  | otherArgs, _ => dbg_trace "Didn't understand {repr otherArgs}"; throwUnsupportedSyntax
 
 end
 
